coq/Progress.v
@@ -4,3 +4,18 @@
 (* 2019 Xuan Huang                                                   *)
 (* ***************************************************************** *)
 
+(* ################################################################# *)
+(** * Progress *)
+
+From Wasm Require Export Validation.
+From Wasm Require Export Execution.
+From Wasm Require Export ExtendedValidation.
+
+Theorem progress : forall S T rt,
+    ⊢c (S, T) ∈ rt ->
+    (* missing Prop to claim instrs are result
+       so we only write take a step here.
+     *)
+    exists S' T', $(S, T) ↪ $(S', T').
+Proof.
+  Abort.
